theories/elpi_equiv.v
@@ -25,7 +25,7 @@ Section NurEqiv.
     + have [fvB fvs] := vars_tree_step_sub_flow vtA vts1 eA.
       have /=vB:= (valid_tree_step vA eA). 
       have {IH}/=:= IH fvB fvs vB; subst.
-      have /=[] := path_atom_exp_cut pA eA => ?; subst.
+      have /=[] := incomplete_exp_cut pA eA => ?; subst.
         have H5 := step_cb_same_subst1 vA eA; subst.
         have [x[tl[H1 [H2 H3]]]] := s2l_CutBrothers s1 [::] vA eA.
         rewrite H1 H2 H5 => IH.
@@ -50,14 +50,14 @@ Section NurEqiv.
       have [[[? SS] H1]] := s2l_Expanded_cut vA eA H; subst.
       rewrite cats0 => ->.
       by apply: CutS.
-    + have vB := valid_tree_next_alt vA nA.
-      have {}fvP := vars_tree_next_alt_sub_flow vtA nA.
+    + have vB := valid_tree_prune vA nA.
+      have {}fvP := vars_tree_prune_sub_flow vtA nA.
       have {IH} /= := IH fvP vts1 vB.
-      by rewrite (next_altF_t2l vA fA nA).
+      by rewrite (pruneF_t2l vA fA nA).
     + move=>/=.
-      rewrite (failed_next_alt_none_t2l _ _ nA)//.
+      rewrite (failed_prune_none_t2l _ _ nA)//.
         by constructor.
-      by apply/next_altFN_fail.
+      by apply/pruneFN_fail.
   Qed.
 
 Lemma elpi_to_tree_aux p v0 a r : 
@@ -72,30 +72,30 @@ Proof.
   - move=> s a fv s1 A vA /= H.
     case fA: (failed A).
       case nA: (prune false A) => [A'|]; last first.
-        by rewrite (failed_next_alt_none_t2l vA fA nA) in H.
-      have /= fA' := next_alt_failedF nA.
-      have /= vA' := (valid_tree_next_alt vA nA).
-      rewrite (next_altF_t2l vA fA nA) in H.
+        by rewrite (failed_prune_none_t2l vA fA nA) in H.
+      have /= fA' := prune_failedF nA.
+      have /= vA' := (valid_tree_prune vA nA).
+      rewrite (pruneF_t2l vA fA nA) in H.
       have [skA ?]:= s2l_empty_hd_success vA' fA' H; subst.
       repeat eexists.
         apply: BackT fA nA _.
         apply: StopT => //.
-      have:=@s2l_next_alt_tl _ s1 nilA vA' skA.
+      have:=@s2l_prune_tl _ s1 nilA vA' skA.
       by rewrite H => ->//; rewrite behead_cons.
     have [skA ?]:= s2l_empty_hd_success vA fA H; subst.
     repeat eexists.
       by apply: StopT.
-    have:=@s2l_next_alt_tl _ s1 nilA vA skA.
+    have:=@s2l_prune_tl _ s1 nilA vA skA.
     by rewrite H => ->//; rewrite behead_cons.
   - move=> s1 a ca r gl fv ELPI IH s A vA H.
     {
       (* CUT CASE *)
       case fA: (failed A).
         case nA: (prune false A) => [A'|]; last first.
-          by rewrite (failed_next_alt_none_t2l vA fA nA) in H.
-        have /= fA' := next_alt_failedF nA.
-        have /= vA' := (valid_tree_next_alt vA nA).
-        rewrite (next_altF_t2l vA fA nA) in H.
+          by rewrite (failed_prune_none_t2l vA fA nA) in H.
+        have /= fA' := prune_failedF nA.
+        have /= vA' := (valid_tree_prune vA nA).
+        rewrite (pruneF_t2l vA fA nA) in H.
         rewrite -(@clean_ca_nil (t2l _ _ _)) in H.
         case X: (step u p fv s A') => [[fv' r'] A''].
         have:= next_cut_s2l fA' vA' H X => /=.
@@ -106,13 +106,13 @@ Proof.
           move: H2; case: ifP => //= CB [??]; subst;
           repeat eexists; apply: BackT fA nA _;
           apply: StepT erefl IH; eauto.
-            by apply: path_atom_cut X.
-          by apply: path_atom_exp X.
+            by apply: incomplete_cut X.
+          by apply: incomplete_exp X.
         move: H2; case: ifP => //= CB [??] IH; subst;
         repeat eexists; apply: BackT fA nA _;
         apply: StepT erefl IH; eauto.
-          by apply: path_atom_cut X.
-        by apply: path_atom_exp X.
+          by apply: incomplete_cut X.
+        by apply: incomplete_exp X.
       rewrite -(@clean_ca_nil (t2l _ _ _)) in H.
       case X: (step u p fv s A) => [[fv' r'] A'].
       have:= next_cut_s2l fA vA H X => /=.
@@ -122,13 +122,13 @@ Proof.
         move=> [t1[IH ?]]; subst.
         move: H2; case: ifP => Hx [??]; subst;
         repeat eexists; apply: StepT (X) erefl IH.
-          by apply: path_atom_cut X.
-        by apply: path_atom_exp X.
+          by apply: incomplete_cut X.
+        by apply: incomplete_exp X.
       move: H2; case: ifP => //= CB [??] IH; subst;
       repeat eexists;
       apply: StepT erefl IH; eauto.
-        by apply: path_atom_cut X.
-      by apply: path_atom_exp X.
+        by apply: incomplete_cut X.
+      by apply: incomplete_exp X.
     }
   - move=> s1 a g bs r t ca fv fv' + ELPI IH s3 A vA H.
     rewrite/stepE; case B: bc => [fv2 rules] [??]; subst.
@@ -136,11 +136,11 @@ Proof.
       (* CALL SUCCESS CASE *)
       case fA: (failed A).
         case nA: (prune false A) => [A'|]; last first.
-          by rewrite (failed_next_alt_none_t2l vA fA nA) in H.
+          by rewrite (failed_prune_none_t2l vA fA nA) in H.
         rewrite -(@clean_ca_nil (t2l _ _ _)) in H.
-        rewrite (next_altF_t2l vA fA nA) in H.
-        have /= fA' := next_alt_failedF nA.
-        have /= vA' := (valid_tree_next_alt vA nA).
+        rewrite (pruneF_t2l vA fA nA) in H.
+        have /= fA' := prune_failedF nA.
+        have /= vA' := (valid_tree_prune vA nA).
         have [] := next_callS_s2l p u fv fA' vA' H.
         rewrite B/=clean_ca_nil => H1 H2.
         have /= {IH}[b[v1]] := IH _ _ (valid_tree_step vA' erefl) H1; subst.
@@ -149,11 +149,11 @@ Proof.
           repeat eexists.
           apply: BackT fA nA _.
           apply: StepT (H2) erefl IH.
-          apply: path_atom_exp H2.
+          apply: incomplete_exp H2.
         move=> IH; repeat eexists.
         apply: BackT fA nA _.
         apply: StepT (H2) erefl IH.
-        apply: path_atom_exp H2.
+        apply: incomplete_exp H2.
       rewrite -(@clean_ca_nil (t2l _ _ _)) in H.
       have [] := next_callS_s2l p u fv fA vA H.
       rewrite B/= clean_ca_nil/= => H1 H2.
@@ -162,11 +162,11 @@ Proof.
         move=> [t'[IH ?]]; subst.
         repeat eexists.
         apply: StepT (H2) erefl IH.
-        apply: path_atom_exp H2.
+        apply: incomplete_exp H2.
       move=> IH.
       repeat eexists.
       apply: StepT (H2) erefl IH.
-      apply: path_atom_exp H2.
+      apply: incomplete_exp H2.
     }
   + by move=> > vT H; repeat eexists; apply/FailT/t2l_nil_na/H.
 Qed.
